Tables/Data/Array/Nodup.lean
@@ -1,0 +1,70 @@
+module
+
+public section
+
+namespace List
+
+variable {α} {l : List α}
+
+-- From Mathlib
+theorem Nodup.filter (p : α → Bool) (h : Nodup l) : Nodup (l.filter p) := by
+  simpa using Pairwise.filter p h
+
+end List
+
+namespace Array
+
+@[expose]
+def Nodup {α} (a : Array α) : Prop :=
+  ∀ i j : Nat, (_ : i < a.size) → (_ : j < a.size) → i ≠ j → a[i] ≠ a[j]
+
+namespace Nodup
+
+theorem empty {α} : Nodup (@empty α) := by
+  intro i j hi hj ne
+  exact (Nat.not_lt_zero i hi).elim
+
+theorem range (n : Nat) : Nodup (Array.range n) := by
+  intro i j
+  simp [Array.getElem_range]
+
+theorem finRange (n : Nat) : Nodup (Array.finRange n) := by
+  intro i j
+  simp [Array.getElem_finRange]
+
+theorem push {α} {a : Array α} {x : α} (h : Nodup a) (hfresh : x ∉ a) : Nodup (a.push x) := by
+  intro i j hi hj ne
+  simp only [getElem_push]
+  split
+  next hi =>
+    split
+    next hj => exact h i j hi hj ne
+    next hj => grind
+  next hi => grind
+
+theorem toList_iff {α} (a : Array α) : a.Nodup ↔ a.toList.Nodup := by
+  constructor
+  . intro h
+    simp only [List.nodup_iff_pairwise_ne, ne_eq, List.pairwise_iff_getElem, length_toList,
+      getElem_toList]
+    intro i j hi hj lt
+    exact h i j hi hj (Nat.ne_of_lt lt)
+  . intro h
+    simp only [List.nodup_iff_pairwise_ne, ne_eq, List.pairwise_iff_getElem, length_toList,
+      getElem_toList] at h
+    intro i j hi hj ne
+    cases Nat.lt_or_gt_of_ne ne with
+    | inl lt => exact h i j hi hj lt
+    | inr gt => exact Ne.symm (h j i hj hi gt)
+
+theorem filter {α} {a : Array α} (p : α → Bool) (h : Nodup a) : Nodup (a.filter p) := by
+  rw [toList_iff, toList_filter]
+  apply List.Nodup.filter p
+  rw [← toList_iff]
+  exact h
+
+end Nodup
+
+end Array
+
+end
